Refine_Imperative_HOL/IICF/Impl/IICF_RbtMap_Map.thy
@@ -144,10 +144,10 @@ definition "map_lookup m k = do {
                   return (the v) }"
  
 
-lemma "x \<in> dom M \<Longrightarrow> M = meval Ma \<Longrightarrow>  v = Ma\<langle>x\<rangle> \<Longrightarrow> xa = the v \<Longrightarrow> xa =
+lemma s[resolve]: "x \<in> dom M \<Longrightarrow> M = meval Ma \<Longrightarrow>  v = Ma\<langle>x\<rangle> \<Longrightarrow> xa = the v \<Longrightarrow> xa =
                      the (M x)"  
   by simp
-   
+
 thm return_rule
 thm SepAuto.return_rule
 theorem map_lookup_rule [hoare_triple]:
@@ -155,8 +155,19 @@ theorem map_lookup_rule [hoare_triple]:
            map_lookup m x  
    <\<lambda>r. rbt_map_map_assn M m * \<up>(r=the (M x))>\<^sub>t"
   unfolding map_dom_member_def
-  sorry (* by auto2 *)
+  apply auto2  sorry
 
+theorem map_lookup_rule [hoare_triple]:
+  "x\<in>dom M \<Longrightarrow> <rbt_map_map_assn M m * $ (rbt_search_time_logN (sizeM1' M)+1)>
+           map_lookup m x  
+   <\<lambda>r. rbt_map_map_assn M m * \<up>(r=the (M x))>\<^sub>t"
+  unfolding map_lookup_def  rbt_map_map_assn_def 
+  apply(rule bind_rule) 
+   apply(rule pre_rule[OF _ frame_rule[OF rbt_search]] )
+  apply(rule match_first)
+  apply(rule frame_rule[OF)
+  unfolding map_dom_member_def
+  apply auto2  oops
 
 
 
